James C - more assembly opcode reworking

AssemblyLanguage.thy
@@ -6,27 +6,29 @@ typedecl symbol
 
 datatype assembly =
   AAssm int
-| SAssm symbol
-| CAssm "register set" computation "comparison set"
+| CAssm "register set" computation
+| JAssm "comparison set" symbol
 
 type_synonym program = "symbol \<leadsto> assembly list"
 
-type_synonym assembly_state = "memory \<times> int \<times> int \<times> symbol \<times> assembly list" (* M, A, D, S, PC *)
+type_synonym assembly_state = "memory \<times> int \<times> int \<times> assembly list" (* M, A, D, PC *)
 
 fun eval_assembly :: "program \<Rightarrow> assembly_state \<Rightarrow> assembly_state option" where
-  "eval_assembly \<Pi> (\<sigma>, a, d, s, []) = None"
-| "eval_assembly \<Pi> (\<sigma>, a, d, s, AAssm x # \<pi>) = Some (\<sigma>, x, d, s, \<pi>)"
-| "eval_assembly \<Pi> (\<sigma>, a, d, s, SAssm x # \<pi>) = Some (\<sigma>, a, d, x, \<pi>)"
-| "eval_assembly \<Pi> (\<sigma>, a, d, s, CAssm dst cmp jmp # \<pi>) = (
+  "eval_assembly \<Pi> (\<sigma>, a, d, []) = None"
+| "eval_assembly \<Pi> (\<sigma>, a, d, AAssm x # \<pi>) = Some (\<sigma>, x, d, \<pi>)"
+| "eval_assembly \<Pi> (\<sigma>, a, d, CAssm dst cmp # \<pi>) = (
     let n = compute cmp (\<sigma> (nat a)) a d
-    in let \<sigma>' = if M \<in> dst then \<sigma>(nat a := n) else \<sigma>
-    in let a' = if A \<in> dst then n else a
-    in let d' = if D \<in> dst then n else d
-    in if should_jump n jmp
-       then case lookup \<Pi> s of 
-           Some \<pi>' \<Rightarrow> Some (\<sigma>', a', d', s, \<pi>')
-         | None \<Rightarrow> None
-       else Some (\<sigma>', a', d', s, \<pi>))"
+    in Some (
+      if M \<in> dst then \<sigma>(nat a := n) else \<sigma>, 
+      if A \<in> dst then n else a, 
+      if D \<in> dst then n else d, 
+      \<pi>))"
+| "eval_assembly \<Pi> (\<sigma>, a, d, JAssm jmp s # \<pi>) = (
+    if should_jump d jmp
+    then case lookup \<Pi> s of 
+        Some \<pi>' \<Rightarrow> Some (\<sigma>, a, d, \<pi>')
+      | None \<Rightarrow> None
+    else Some (\<sigma>, a, d, \<pi>))"
 
 (* conversion *)
 
@@ -39,37 +41,22 @@ fun build_symbol_table :: "program \<Rightarrow> symbol \<rightharpoonup> nat" w
 definition get_block_addr :: "(symbol \<rightharpoonup> nat) \<Rightarrow> symbol \<Rightarrow> int" where
   "get_block_addr \<rho> s = int (the (\<rho> s))"
 
-primrec instruction_conv :: "(symbol \<rightharpoonup> nat) \<Rightarrow> assembly \<Rightarrow> instruction" where
-  "instruction_conv \<rho> (AAssm x) = AInstr x"
-| "instruction_conv \<rho> (SAssm x) = AInstr (get_block_addr \<rho> x)"
-| "instruction_conv \<rho> (CAssm dst cmp jmp) = CInstr dst cmp jmp"
+primrec instruction_conv :: "(symbol \<rightharpoonup> nat) \<Rightarrow> assembly \<Rightarrow> instruction list" where
+  "instruction_conv \<rho> (AAssm x) = [AInstr x]"
+| "instruction_conv \<rho> (CAssm dst cmp) = [CInstr dst cmp {}]"
+| "instruction_conv \<rho> (JAssm jmp s) = [AInstr (get_block_addr \<rho> s), CInstr {} (Reg D) jmp]"
 
 definition get_assembly :: "program \<Rightarrow> assembly list" where
   "get_assembly \<Pi> = concat (map snd \<Pi>)"
 
 definition program_convert :: "program \<Rightarrow> instruction list" where
-  "program_convert \<Pi> = map (instruction_conv (build_symbol_table \<Pi>)) (get_assembly \<Pi>)"
-
-(* conversion safety typecheck *)
-
-datatype acc_type = Number | Symbol
-
-fun typecheck_assembly :: "assembly list \<Rightarrow> acc_type \<Rightarrow> bool" where
-  "typecheck_assembly [] t = True"
-| "typecheck_assembly (AAssm x # \<pi>) t = typecheck_assembly \<pi> Number"
-| "typecheck_assembly (SAssm x # \<pi>) t = typecheck_assembly \<pi> Symbol"
-| "typecheck_assembly (CAssm dst cmp jmp # \<pi>) Number = (jmp = {} \<and> typecheck_assembly \<pi> Number)"
-| "typecheck_assembly (CAssm dst cmp jmp # \<pi>) Symbol = (dst = {} \<and> typecheck_assembly \<pi> Symbol)"
-
-definition typecheck_program :: "program \<Rightarrow> bool" where
-  "typecheck_program \<Pi> = (\<forall>\<pi> \<in> ran (lookup \<Pi>). typecheck_assembly \<pi> Symbol)"
+  "program_convert \<Pi> = concat (map (instruction_conv (build_symbol_table \<Pi>)) (get_assembly \<Pi>))"
 
 definition get_pc :: "program \<Rightarrow> assembly list \<Rightarrow> nat set" where
   "get_pc \<Pi> \<pi> = { the (build_symbol_table \<Pi> s) + length \<pi>' | s \<pi>'. lookup \<Pi> s = Some (\<pi>' @ \<pi>) }"
 
 fun state_convert :: "program \<Rightarrow> assembly_state \<Rightarrow> machine_state set" where
-  "state_convert \<Pi> (\<sigma>, a, d, s, \<pi>) = (\<lambda>pc. (\<sigma>, a, d, pc)) ` get_pc \<Pi> \<pi> \<union> 
-    (\<lambda>pc. (\<sigma>, get_block_addr (build_symbol_table \<Pi>) s, d, pc)) ` get_pc \<Pi> \<pi>"
+  "state_convert \<Pi> (\<sigma>, a, d, \<pi>) = (\<lambda>pc. (\<sigma>, a, d, pc)) ` get_pc \<Pi> \<pi>"
 
 (* conversion correctness *)
 
@@ -92,6 +79,12 @@ lemma [simp]: "lookup \<Pi> s = Some \<pi> \<Longrightarrow> n < length \<pi> \<
       qed
   qed
 
+lemma [simp]: "1 \<le> length (instruction_conv \<rho> a)"
+  by (induction a) simp_all
+
+lemma [simp]: "length \<pi> \<le> length (concat (map (instruction_conv \<rho>) \<pi>))"
+  apply (induction \<pi>) apply simp_all by simp
+
 lemma [simp]: "lookup \<Pi> s = Some (\<pi> @ \<pi>') \<Longrightarrow> \<pi>' \<noteq> [] \<Longrightarrow>
     the (build_symbol_table \<Pi> s) + length \<pi> < length (program_convert \<Pi>)"
   proof (induction \<Pi> s rule: build_symbol_table.induct)
@@ -101,7 +94,7 @@ lemma [simp]: "lookup \<Pi> s = Some (\<pi> @ \<pi>') \<Longrightarrow> \<pi>' \
     thus ?case
       proof (cases "s' = s")
       case True
-        with 2 show ?thesis by (simp add: program_convert_def get_assembly_def)
+        with 2 show ?thesis apply (simp add: program_convert_def get_assembly_def) by simp
       next case False
         with 2 obtain m where "build_symbol_table \<Pi> s = Some m" by fastforce
         with 2 False show ?thesis by (simp add: program_convert_def get_assembly_def)
@@ -124,8 +117,8 @@ lemma [simp]: "lookup \<Pi> s = Some \<pi> \<Longrightarrow> n < length \<pi> \<
       qed
   qed
 
-lemma [simp]: "pc \<in> get_pc \<Pi> (a # \<pi>) \<Longrightarrow> 
-    program_convert \<Pi> ! pc = instruction_conv (build_symbol_table \<Pi>) a"
+lemma [simp]: "pc \<in> get_pc \<Pi> (a # \<pi>) \<Longrightarrow> i < length (instruction_conv (build_symbol_table \<Pi>) a) \<Longrightarrow>
+    program_convert \<Pi> ! (pc + i) = instruction_conv (build_symbol_table \<Pi>) a ! i"
   by (auto simp add: get_pc_def program_convert_def)
 
 lemma [simp]: "pc \<in> get_pc \<Pi> (a # \<pi>) \<Longrightarrow> pc < length (program_convert \<Pi>)"
@@ -141,32 +134,31 @@ lemma [simp]: "pc \<in> get_pc \<Pi> (a # \<pi>) \<Longrightarrow> Suc pc \<in> 
     with P show "Suc pc \<in> get_pc \<Pi> \<pi>" by (simp add: get_pc_def)
   qed
 
-lemma eval_assembly_conv [simp]: "eval_assembly \<Pi> \<sigma> = Some \<sigma>\<^sub>1 \<Longrightarrow> \<sigma>' \<in> state_convert \<Pi> \<sigma> \<Longrightarrow>
-    typecheck_program \<Pi> \<Longrightarrow> 
-      \<exists>\<sigma>\<^sub>1'. \<sigma>\<^sub>1' \<in> state_convert \<Pi> \<sigma>\<^sub>1 \<and> eval (program_convert \<Pi>) \<sigma>' = Some \<sigma>\<^sub>1'"
-  proof (induction \<Pi> \<sigma> rule: eval_assembly.induct)
+lemma eval_assembly_conv [simp]: "eval_assembly \<Pi> \<Sigma> = Some \<Sigma>\<^sub>1 \<Longrightarrow> \<Sigma>' \<in> state_convert \<Pi> \<Sigma> \<Longrightarrow>
+    \<exists>\<Sigma>\<^sub>1'. \<Sigma>\<^sub>1' \<in> state_convert \<Pi> \<Sigma>\<^sub>1 \<and> eval (program_convert \<Pi>) \<Sigma>' = Some \<Sigma>\<^sub>1'"
+  proof (induction \<Pi> \<Sigma> rule: eval_assembly.induct)
   case 1
     thus ?case by simp
   next case 2
-    thus ?case by auto
+    thus ?case by simp
   next case 3
-    thus ?case by auto
-  next case (4 \<Pi> \<sigma> a d s dst cmp jmp \<pi>)
-    thus ?case by auto
+    thus ?case by simp
+  next case 4
+    thus ?case by simp
   qed
 
-theorem [simp]: "iterate (eval_assembly \<Pi>) \<sigma> \<sigma>\<^sub>1 \<Longrightarrow> \<sigma>' \<in> state_convert \<Pi> \<sigma> \<Longrightarrow> 
-    typecheck_program \<Pi> \<Longrightarrow> 
-      \<exists>\<sigma>\<^sub>1'. \<sigma>\<^sub>1' \<in> state_convert \<Pi> \<sigma>\<^sub>1 \<and> iterate (eval (program_convert \<Pi>)) \<sigma>' \<sigma>\<^sub>1'"
-  proof (induction "eval_assembly \<Pi>" \<sigma> \<sigma>\<^sub>1 arbitrary: \<sigma>' rule: iterate.induct)
+theorem [simp]: "iterate (eval_assembly \<Pi>) \<Sigma> \<Sigma>\<^sub>1 \<Longrightarrow> \<Sigma>' \<in> state_convert \<Pi> \<Sigma> \<Longrightarrow> 
+    \<exists>\<Sigma>\<^sub>1'. \<Sigma>\<^sub>1' \<in> state_convert \<Pi> \<Sigma>\<^sub>1 \<and> iterate (eval (program_convert \<Pi>)) \<Sigma>' \<Sigma>\<^sub>1'"
+  proof (induction "eval_assembly \<Pi>" \<Sigma> \<Sigma>\<^sub>1 arbitrary: \<Sigma>' rule: iterate.induct)
   case iter_refl
     thus ?case by fastforce
-  next case (iter_step \<sigma> \<sigma>\<^sub>1 \<sigma>\<^sub>2)
-    then obtain \<sigma>\<^sub>1' where S: "\<sigma>\<^sub>1' \<in> state_convert \<Pi> \<sigma>\<^sub>1 \<and> iterate (eval (program_convert \<Pi>)) \<sigma>' \<sigma>\<^sub>1'" 
-      by blast
-    with iter_step eval_assembly_conv obtain \<sigma>\<^sub>2' where
-      "\<sigma>\<^sub>2' \<in> state_convert \<Pi> \<sigma>\<^sub>2 \<and> eval (program_convert \<Pi>) \<sigma>\<^sub>1' = Some \<sigma>\<^sub>2'" by blast
-    with S have "\<sigma>\<^sub>2' \<in> state_convert \<Pi> \<sigma>\<^sub>2 \<and> iterate (eval (program_convert \<Pi>)) \<sigma>' \<sigma>\<^sub>2'" by fastforce
+  next case (iter_step \<Sigma> \<Sigma>\<^sub>1 \<Sigma>\<^sub>2)
+    then obtain \<Sigma>\<^sub>1' where S: "\<Sigma>\<^sub>1' \<in> state_convert \<Pi> \<Sigma>\<^sub>1 \<and> 
+      iterate (eval (program_convert \<Pi>)) \<Sigma>' \<Sigma>\<^sub>1'" by blast
+    with iter_step eval_assembly_conv obtain \<Sigma>\<^sub>2' where
+      "\<Sigma>\<^sub>2' \<in> state_convert \<Pi> \<Sigma>\<^sub>2 \<and> eval (program_convert \<Pi>) \<Sigma>\<^sub>1' = Some \<Sigma>\<^sub>2'" by blast
+    with S have "\<Sigma>\<^sub>2' \<in> state_convert \<Pi> \<Sigma>\<^sub>2 \<and> iterate (eval (program_convert \<Pi>)) \<Sigma>' \<Sigma>\<^sub>2'" 
+      by fastforce
     thus ?case by blast
   qed
 
